Of course, here is the solution to question Q2.

### **Problem Statement**

Let the integral be defined for any natural number n ≥ 1:
Aₙ = ∫₀¹ (1 - x²) xⁿ⁻¹ dx

Compute A₁ + A₂.

### **Step 1: Calculate A₁**

To find A₁, we set n = 1 in the given formula:

A₁ = ∫₀¹ (1 - x²) x¹⁻¹ dx
A₁ = ∫₀¹ (1 - x²) x⁰ dx
A₁ = ∫₀¹ (1 - x²) dx

Now, we evaluate the integral:
A₁ = [x - (x³/3)] from 0 to 1
A₁ = (1 - 1³/3) - (0 - 0³/3)
A₁ = (1 - 1/3) - 0
**A₁ = 2/3**

### **Step 2: Calculate A₂**

To find A₂, we set n = 2 in the given formula:

A₂ = ∫₀¹ (1 - x²) x²⁻¹ dx
A₂ = ∫₀¹ (1 - x²) x¹ dx
A₂ = ∫₀¹ (x - x³) dx

Now, we evaluate the integral:
A₂ = [(x²/2) - (x⁴/4)] from 0 to 1
A₂ = (1²/2 - 1⁴/4) - (0²/2 - 0⁴/4)
A₂ = (1/2 - 1/4) - 0
**A₂ = 1/4**

### **Step 3: Compute A₁ + A₂**

Finally, we add the values of A₁ and A₂:

A₁ + A₂ = 2/3 + 1/4

To add these fractions, we find a common denominator, which is 12:

A₁ + A₂ = (8/12) + (3/12)
**A₁ + A₂ = 11/12**
